CATCH for exceptions. Example how to use this as break!

Snippets.thy
@@ -2,7 +2,7 @@ theory Snippets
 imports VTcomp
 begin
 
-  (** Plain arrays *)
+  section \<open>Find Element in Array (Arrays)\<close>
 
   definition "find_elem (x::int) xs \<equiv> do {
     WHILEIT (\<lambda>i. i\<le>length xs \<and> x\<notin>set (take i xs)) (\<lambda>i. i<length xs \<and> xs!i\<noteq>x) (\<lambda>i. RETURN (i+1)) 0
@@ -23,7 +23,8 @@ begin
   export_code find_elem_impl in Haskell module_name test
 
 
-  
+  section \<open>Check Prefix (Arrays, Exceptions: Check)\<close>
+    
   definition "check_prefix xs ys \<equiv> doE {
     CHECK (length xs \<le> length ys) ();
     EWHILEIT (\<lambda>i. i\<le>length xs \<and> take i xs = take i ys) (\<lambda>i. i<length xs) (\<lambda>i. doE { 
@@ -70,6 +71,63 @@ begin
   export_code check_prefix_impl checking SML_imp
   
 
+  section \<open>Is Prefix (Arrays, Exceptions: Catch)\<close>
+  
+  definition "is_prefix xs ys \<equiv> CATCH (doE {
+    CHECK (length xs \<le> length ys) ();
+    EWHILEIT (\<lambda>i. i\<le>length xs \<and> take i xs = take i ys) (\<lambda>i. i<length xs) (\<lambda>i. doE { 
+      EASSERT (i<length xs \<and> i<length ys); 
+      CHECK (xs!i = ys!i) (); 
+      ERETURN (i+1) 
+    } ) 0;
+    ERETURN True
+  }) (\<lambda>_. ERETURN False)"
+  
+  (* ESPEC Exc Normal ! *)
+  lemma "is_prefix xs ys \<le> ESPEC (\<lambda>_. False) (\<lambda>r. r \<longleftrightarrow> xs = take (length xs) ys)"
+    unfolding is_prefix_def
+    apply (refine_vcg EWHILEIT_rule[where R="measure (\<lambda>i. length xs - i)"])
+    apply auto []
+    apply auto []
+    apply auto []
+    apply auto []
+    apply auto []
+    apply auto []
+    subgoal
+      by (simp add: take_Suc_conv_app_nth)
+    apply auto []
+    apply auto []
+    subgoal 
+      by (metis nth_take)
+    subgoal 
+      by force
+    apply auto []
+    done
+  
+  synth_definition is_prefix_bd is [enres_unfolds]: "is_prefix xs ys = \<hole>"
+    apply (rule CNV_eqD)
+    unfolding is_prefix_def
+    apply opt_enres_unfold
+    apply (rule CNV_I)
+    done
+    
+  sepref_definition is_prefix_impl is "uncurry is_prefix_bd" 
+    :: "(array_assn int_assn)\<^sup>k *\<^sub>a (array_assn int_assn)\<^sup>k \<rightarrow>\<^sub>a (unit_assn +\<^sub>a bool_assn)"
+    unfolding is_prefix_bd_def
+    by sepref
+  
+  export_code is_prefix_impl checking SML_imp
+  
+  
+  
+  
+  
+  
+  
+  
+  
+  section \<open>Copy Array (Arrays, For i=l..u)\<close>  
+  
   definition "cp_array xs \<equiv> do {
     let ys = op_array_replicate (length xs) 0;   (* Use proper constructors *)
     
